James C - completed parsing, getting into parse-correctness

Jack/JackLanguage.thy
@@ -18,7 +18,7 @@ datatype binop =
 datatype expression =
   IConst int
 | BConst bool
-| CConst char
+| SConst string
 | Var variable
 | This 
 | Null
@@ -56,65 +56,60 @@ record classdecl =
 
 datatype program = Program "(variable \<times> classdecl) list" "statement list"
 
-(* typechecking *)
+(* printing *)
 
-inductive typecheck_binop :: "binop \<Rightarrow> type \<Rightarrow> type \<Rightarrow> bool" where
-  tc_plus [simp]: "typecheck_binop Plus IntT IntT"
-| tc_minus [simp]: "typecheck_binop Minus IntT IntT"
-| tc_times [simp]: "typecheck_binop Times IntT IntT"
-| tc_div [simp]: "typecheck_binop Div IntT IntT"
-| tc_and [simp]: "typecheck_binop And BoolT BoolT"
-| tc_or [simp]: "typecheck_binop Or BoolT BoolT"
-| tc_eqi [simp]: "typecheck_binop Eq IntT BoolT"
-| tc_eqc [simp]: "typecheck_binop Eq CharT BoolT"
-| tc_eqb [simp]: "typecheck_binop Eq BoolT BoolT"
-| tc_gt [simp]: "typecheck_binop Gt IntT BoolT"
-| tc_lt [simp]: "typecheck_binop Lt IntT BoolT"
+definition combine_with_space :: "string \<Rightarrow> string \<Rightarrow> string" where
+  "combine_with_space s\<^sub>1 s\<^sub>2 = s\<^sub>1 @ ''\<newline>'' @ s\<^sub>2"
 
-inductive typecheck_expr :: "(variable \<rightharpoonup> type) \<Rightarrow> type \<Rightarrow> expression \<Rightarrow> type \<Rightarrow> bool" where
-  "typecheck_expr \<Gamma> this (IConst i) IntT"
-| "typecheck_expr \<Gamma> this (BConst b) BoolT"
-| "typecheck_expr \<Gamma> this (CConst b) CharT"
-| "\<Gamma> x = Some t \<Longrightarrow> typecheck_expr \<Gamma> this (Var x) t"
-| "typecheck_expr \<Gamma> this This this"
-| "typecheck_expr \<Gamma> this Null (ObjT tx)"
-| "typecheck_expr \<Gamma> this e1 (ArrayT t) \<Longrightarrow> typecheck_expr \<Gamma> this e2 IntT \<Longrightarrow> 
-    typecheck_expr \<Gamma> this (Index e1 e2) t"
-| "typecheck_expr \<Gamma> this e (ObjT tx) \<Longrightarrow> badbadbad x = Some t \<Longrightarrow> typecheck_expr \<Gamma> this (Field e x) t"
-| "typecheck_expr \<Gamma> this e (ObjT tx) \<Longrightarrow> badbadbad x = Some (ArrowT ts t) \<Longrightarrow> 
-    \<forall>(e', t') \<in> set (zip es ts). typecheck_expr \<Gamma> this e' t' \<Longrightarrow> 
-      typecheck_expr \<Gamma> this (Call e x es) t"
-| "typecheck_expr \<Gamma> this e IntT \<Longrightarrow> typecheck_expr \<Gamma> this (Negate e) IntT"
-| "typecheck_expr \<Gamma> this e BoolT \<Longrightarrow> typecheck_expr \<Gamma> this (Not e) BoolT"
-| "typecheck_binop b t1 t2 \<Longrightarrow> typecheck_expr \<Gamma> this e1 t1 \<Longrightarrow> typecheck_expr \<Gamma> this e2 t1 \<Longrightarrow> 
-    typecheck_expr \<Gamma> this (Binop b e1 e2) t2"
+definition combine_with_comma :: "string \<Rightarrow> string \<Rightarrow> string" where
+  "combine_with_comma s\<^sub>1 s\<^sub>2 = s\<^sub>1 @ '' , '' @ s\<^sub>2"
 
-inductive typecheck_lval :: "(variable \<rightharpoonup> type) \<Rightarrow> type \<Rightarrow> lvar \<Rightarrow> type \<Rightarrow> bool" where
-  "\<Gamma> x = Some t \<Longrightarrow> typecheck_lval \<Gamma> this (LVar x) t"
-| "typecheck_lval \<Gamma> this l1 (ArrayT t) \<Longrightarrow> typecheck_expr \<Gamma> this e2 IntT \<Longrightarrow> 
-    typecheck_lval \<Gamma> this (LIndex l1 e2) t"
-| "typecheck_lval \<Gamma> this e (ObjT tx) \<Longrightarrow> badbadbad x = Some t \<Longrightarrow> typecheck_lval \<Gamma> this (LField e x) t"
+primrec type_to_string :: "type \<Rightarrow> string" where
+  "type_to_string IntT = ''int''"
+| "type_to_string BoolT = ''bool''"
+| "type_to_string CharT = ''char''"
+| "type_to_string UnitT = ''void''"
+| "type_to_string (ObjT x) = ''x''"
+| "type_to_string (ArrayT t) = ''array of '' @ type_to_string t"
+| "type_to_string (ArrowT t1 t2) = 
+    foldl combine_with_comma ''['' (map type_to_string t1) @ ''] => '' @ type_to_string t2"
 
-inductive typecheck_stmt :: "(variable \<rightharpoonup> type) \<Rightarrow> type \<Rightarrow> type \<Rightarrow> statement \<Rightarrow> bool" where
-  "typecheck_lval \<Gamma> this x t \<Longrightarrow> typecheck_expr \<Gamma> this e t \<Longrightarrow> typecheck_stmt \<Gamma> this out (Let x e)"
-| "typecheck_expr \<Gamma> this e BoolT \<Longrightarrow> \<forall>s' \<in> set s1. typecheck_stmt \<Gamma> this out s' \<Longrightarrow> 
-    \<forall>s' \<in> set s2. typecheck_stmt \<Gamma> this out s' \<Longrightarrow> typecheck_stmt \<Gamma> this out (If e s1 s2)"
-| "typecheck_expr \<Gamma> this e BoolT \<Longrightarrow> \<forall>s' \<in> set s. typecheck_stmt \<Gamma> this out s' \<Longrightarrow> 
-    typecheck_stmt \<Gamma> this out (While e s)"
-| "typecheck_expr \<Gamma> this e (ObjT tx) \<Longrightarrow> badbadbad x = Some (ArrowT ts UnitT) \<Longrightarrow> 
-    \<forall>(e', t') \<in> set (zip es ts). typecheck_expr \<Gamma> this e' t' \<Longrightarrow> 
-      typecheck_stmt \<Gamma> this out (Do e x es)"
-| "typecheck_expr \<Gamma> this e out \<Longrightarrow> typecheck_stmt \<Gamma> this out (Return e)"
+primrec binop_to_string :: "binop \<Rightarrow> string" where
+  "binop_to_string Plus = ''+''"
+| "binop_to_string Minus = ''-''"
+| "binop_to_string Times = ''*''"
+| "binop_to_string Div = ''/''"
+| "binop_to_string And = ''&''"
+| "binop_to_string Or = ''|''"
+| "binop_to_string Eq = ''=''"
+| "binop_to_string Lt = ''<''"
+| "binop_to_string Gt = ''>''"
 
-inductive typecheck_subr :: "(variable \<rightharpoonup> type) \<Rightarrow> type \<Rightarrow> subroutine \<Rightarrow> bool" where
-  "\<forall>s \<in> set sts. typecheck_stmt (\<Gamma> ++ map_of ps ++ map_of ls) this t s \<Longrightarrow> 
-    typecheck_subr \<Gamma> this \<lparr> outtype = t, params = ps, locals = ls, body = sts \<rparr>"
+primrec expression_to_string :: "expression \<Rightarrow> string" where
+  "expression_to_string (IConst i) = ''i''"
+| "expression_to_string (BConst b) = (if b then ''true'' else ''false'')"
+| "expression_to_string (SConst s) = ''\"'' @ s @ ''\"''"
+| "expression_to_string (Var x) = x"
+| "expression_to_string This = ''this''"
+| "expression_to_string Null = ''null''"
 
-inductive typecheck_class :: "classdecl \<Rightarrow> bool" where
-  "typecheck_class \<lparr> staticvars = svs, instancevars = ivs, staticfuncs = sfs, constructors = cts, instancefuncs = ifs \<rparr>"
+primrec lvar_to_string :: "lvar \<Rightarrow> string" where
+  "lvar_to_string (LVar x) = x"
 
-inductive typecheck_program :: "program \<Rightarrow> bool" where
-  "\<forall>(n, cl) \<in> set classes. typecheck_class cl \<Longrightarrow> \<forall>s \<in> set main. typecheck_stmt \<Gamma> this t s \<Longrightarrow> 
-    typecheck_program (Program classes main)"
+primrec statement_to_string :: "statement \<Rightarrow> string" where
+  "statement_to_string (Let x e) = ''let '' @ lvar_to_string x @ '' = '' @ expression_to_string e"
+
+fun subroutine_to_string :: "subroutine \<Rightarrow> string" where
+  "subroutine_to_string \<lparr> outtype = out, params = ps, locals = ls, body = b \<rparr> = undefined"
+
+primrec vardecl_to_string :: "(variable \<times> type) \<Rightarrow> string" where
+  "vardecl_to_string (x, t) = type_to_string t @ '' '' @ x"
+
+fun classdecl_to_string :: "(variable \<times> classdecl) \<Rightarrow> string" where
+  "classdecl_to_string (name, cl) = ''class { '' @ undefined @ ''}''"
+
+primrec program_to_string :: "program \<Rightarrow> string" where
+  "program_to_string (Program classes main) = 
+    foldl combine_with_space [] (map classdecl_to_string classes)"
 
 end
