Jack/ParsingCorrectness.thy
@@ -1,0 +1,16 @@
+theory ParsingCorrectness
+imports JackParsing
+begin
+
+
+
+
+
+
+
+
+theorem parse_correct: "complete_jack_parser (program_to_string \<Pi>) = Some \<Pi>"
+  apply (induction \<Pi>)
+  by simp
+
+end
